we actually don't need the explicit output in round

Clean/Gadgets/BLAKE3/Round.lean
@@ -29,39 +29,15 @@ def main (input : Var Inputs (F p)) : Circuit (F p) (Var BLAKE3State (F p)) := d
   let state ← subcircuit (G.circuit 1 6 11 12) ⟨state, message[10], message[11]⟩
   let state ← subcircuit (G.circuit 2 7 8 13) ⟨state, message[12], message[13]⟩
   let state ← subcircuit (G.circuit 3 4 9 14) ⟨state, message[14], message[15]⟩
-
-  -- TODO: this last copy is unnecessary, however if it not copied
-  -- the output is a mess to deal with in subsequent circuits
-  let state <== state
   return state
 
 -- #eval! main (p:=pBabybear) default |>.localLength
 -- #eval! main (p:=pBabybear) default |>.output
 instance elaborated : ElaboratedCircuit (F p) Inputs BLAKE3State where
   main := main
-  localLength _ := 832
+  localLength _ := 768
   localLength_eq input i0 := by
     simp only [main, circuit_norm, G.circuit, subcircuit_norm, G.elaborated]
-
-  output input i0 := varFromOffset BLAKE3State (i0 + 768)
-  output_eq := by
-    intros
-    dsimp [main, circuit_norm, G.circuit]
-
-  subcircuitsConsistent := by
-    intros
-    dsimp only [main, Fin.isValue, G.circuit, HasAssignEq.assign_eq, HasAssertEq.assert_eq,
-      assertEquals, Circuit.pure_def, Circuit.bind_def, assertion.eq_1, List.cons_append,
-      List.nil_append, ProvableType.witness.eq_1, size, Nat.reduceMul, Operations.localLength.eq_2,
-      Operations.localLength.eq_1, Nat.add_zero, subcircuit.eq_1, ElaboratedCircuit.output,
-      Fin.coe_ofNat_eq_mod, Nat.reduceMod, Operations.localLength.eq_5,
-      Circuit.subcircuit_localLength_eq, ElaboratedCircuit.localLength, Fin.val_two, Fin.val_one,
-      Fin.val_zero, Circuit.operations, Operations.SubcircuitsConsistent.eq_1,
-      Operations.forAll.eq_5, Operations.forAll.eq_2, Circuit.assertion_localLength_eq,
-      ↓Equality.elaborated_eq, Operations.forAll.eq_1]
-    simp only [and_true, true_and]
-    (repeat' constructor) <;> ac_rfl
-
 
 
 def Assumptions (input : Inputs (F p)) :=
@@ -80,55 +56,37 @@ theorem soundness : Soundness (F p) elaborated Assumptions Spec := by
   obtain ⟨h_state, h_message⟩ := h_normalized
   obtain ⟨h_eval_state, h_eval_message⟩ := h_input
 
-  dsimp only [ElaboratedCircuit.main, main, Fin.isValue, G.circuit, G.elaborated,
+  dsimp only [ElaboratedCircuit.main, main, Fin.isValue, G.circuit, G.elaborated, Fin.val_zero,
     Fin.coe_ofNat_eq_mod, Nat.reduceMod, Rotation32.output, Fin.reduceMod, Nat.cast_ofNat,
-    HasAssignEq.assign_eq, HasAssertEq.assert_eq, assertEquals, Circuit.pure_def, Circuit.bind_def,
-    assertion.eq_1, FormalAssertion.toSubcircuit.eq_1, ↓Equality.elaborated_eq, Circuit.operations,
-    ElaboratedCircuit.localLength, Environment.ExtendsVector.eq_1, List.cons_append,
-    List.nil_append, ProvableType.witness.eq_1, size, Nat.reduceMul, Operations.localLength.eq_2,
-    Operations.localLength.eq_1, Nat.add_zero, subcircuit.eq_1, ElaboratedCircuit.output,
-    FormalCircuit.toSubcircuit.eq_1, Operations.localLength.eq_5,
-    Circuit.ConstraintsHold.Soundness.eq_5, Circuit.ConstraintsHold.Soundness.eq_2,
+    Fin.val_one, Fin.val_two, pure, Circuit.bind_def, subcircuit.eq_1, ElaboratedCircuit.output,
+    FormalCircuit.toSubcircuit.eq_1, Circuit.operations, ElaboratedCircuit.localLength,
+    List.cons_append, List.nil_append, Operations.localLength.eq_5, Operations.localLength.eq_1,
+    Nat.add_zero, Circuit.ConstraintsHold.Soundness.eq_5,
     Circuit.ConstraintsHold.Soundness.eq_1] at h_holds
   simp only [G.Assumptions, ↓ProvableStruct.eval_eq_eval, ProvableStruct.eval, fromComponents,
     ProvableStruct.eval.go, h_eval_state, getElem_eval_vector, h_eval_message, G.Spec, Fin.isValue,
-    Nat.cast_zero, and_imp, Equality.circuit, forall_const, and_true] at h_holds
-  obtain ⟨c1, c2, c3, c4, c5, c6, c7, c8, c9⟩ := h_holds
+    Nat.cast_zero, and_imp, and_true] at h_holds
+  obtain ⟨c1, c2, c3, c4, c5, c6, c7, c8⟩ := h_holds
   simp_all only [forall_const]
 
   -- resolve chain of assumptions
   specialize c1 (h_message 0) (h_message 1)
   rw [c1.left] at c2
   specialize c2 c1.right (h_message 2) (h_message 3)
-  clear c1
-
   rw [c2.left] at c3
   specialize c3 c2.right (h_message 4) (h_message 5)
-  clear c2
-
   rw [c3.left] at c4
   specialize c4 c3.right (h_message 6) (h_message 7)
-  clear c3
-
   rw [c4.left] at c5
   specialize c5 c4.right (h_message 8) (h_message 9)
-  clear c4
-
   rw [c5.left] at c6
   specialize c6 c5.right (h_message 10) (h_message 11)
-  clear c5
-
   rw [c6.left] at c7
   specialize c7 c6.right (h_message 12) (h_message 13)
-  clear c6
-
   rw [c7.left] at c8
   specialize c8 c7.right (h_message 14) (h_message 15)
-  clear c7
 
-  -- TODO for some reason `circuit_norm` dos not apply automatically this thm
-  rw [eval_pair (α := BLAKE3State) (β := BLAKE3State) env] at c9
-  simp [circuit_norm] at c9
+  clear c1 c2 c3 c4 c5 c6 c7
 
   -- now c8 is basically the goal
   simp only [Spec, ElaboratedCircuit.output, Circuit.output, main, G.circuit, G.elaborated,
@@ -142,9 +100,8 @@ theorem soundness : Soundness (F p) elaborated Assumptions Spec := by
     List.length_cons, List.length_nil, zero_add, Nat.reduceAdd, List.foldl_toArray',
     List.foldl_cons, List.foldl_nil]
   constructor
-  · rw [c9, c8.left]
-  · rw [c9]
-    exact c8.right
+  · rw [←c8.left]; rfl
+  · exact c8.right
 
 theorem completeness : Completeness (F p) elaborated Assumptions := by
   rintro i0 env ⟨state_var, message_var⟩ henv ⟨state, message⟩ h_input h_normalized
@@ -162,7 +119,7 @@ theorem completeness : Completeness (F p) elaborated Assumptions := by
 
   rw [h_input.left, h_input.right] at henv
   simp [Assumptions] at h_normalized
-  obtain ⟨c1, c2, c3, c4, c5, c6, c7, c8, c9⟩ := henv
+  obtain ⟨c1, c2, c3, c4, c5, c6, c7, c8⟩ := henv
 
 
   specialize c1 h_normalized.left (h_normalized.right 0) (h_normalized.right 1)
@@ -175,17 +132,15 @@ theorem completeness : Completeness (F p) elaborated Assumptions := by
   specialize c8 c7.right (h_normalized.right 14) (h_normalized.right 15)
 
   simp only [Fin.isValue, c1.right, true_and, c2.right, c3.right, c4.right, c5.right, c6.right,
-    c7.right, c8.left, c9]
-
+    c7.right]
   clear c1 c2 c3 c4 c5 c6 c7 c8
 
   rw [h_input.left]
   simp only [Fin.forall_fin_succ, Fin.isValue, Fin.val_zero, Fin.val_succ, zero_add, Nat.reduceAdd,
     Fin.val_eq_zero, IsEmpty.forall_iff, and_true] at h_normalized
 
-  simp [h_normalized, getElem_eval_vector, h_input.right, and_self, true_and]
+  simp only [h_normalized, getElem_eval_vector, h_input.right, and_self]
 
-  sorry
 
 def circuit : FormalCircuit (F p) Inputs BLAKE3State := {
   elaborated with Assumptions, Spec, soundness, completeness
